compile

theories/LambdaWP.v
@@ -54,14 +54,14 @@ Definition wp_triple_ E t :=
 
 
 (* ---------------------------------------------------------------------- *)
-(* ** Definition of [local] for WP *)
+(* ** Definition of [flocal] for WP *)
 
-(** [local F] transforms a weakestpre formula [F], e.g. of the form [wp_triple t],
+(** [flocal F] transforms a weakestpre formula [F], e.g. of the form [wp_triple t],
     into a logically-equivalent formula that smoothly supports applications
     of the structural rule of Separation Logic. The definition is:
 
 [[
-Definition local (F:formula) : formula :=
+Definition flocal (F:formula) : formula :=
   fun Q => \exists Q', F Q' \* (Q' \--* (Q \*+ \Top)).
 ]]
 
@@ -70,7 +70,7 @@ Definition local (F:formula) : formula :=
    that [F] be logically equivalent to [is_local F].
 
 [[
-Definition is_local (F:formula) :=
+Definition is_flocal (F:formula) :=
   F = local F.
 ]]
 
@@ -82,156 +82,156 @@ Definition is_local (F:formula) :=
 
 Definition formula_ (B:Type) := (B -> hprop) -> hprop.
 
-(** The [local] predicate is a predicate transformer that typically
+(** The [flocal] predicate is a predicate transformer that typically
    applies to a WP, and allows for application
    of the frame rule, of the rule of consequence, of the garbage
    collection rule, and of extraction rules for existentials and
    pure facts. *)
 
-Definition local B (F:formula_ B) : formula_ B :=
+Definition flocal B (F:formula_ B) : formula_ B :=
   fun Q => \exists Q', F Q' \* (Q' \--* (Q \*+ \Top)).
 
-(** The [is_local] predicate asserts that a predicate is subject
-  to all the rules that the [local] predicate transformer supports. *)
+(** The [is_flocal] predicate asserts that a predicate is subject
+  to all the rules that the [flocal] predicate transformer supports. *)
 
-Definition is_local B (F:formula_ B) :=
-  F = local F.
+Definition is_flocal B (F:formula_ B) :=
+  F = flocal F.
 
-(** [is_local_pred S] asserts that [is_local (S x)] holds for any [x].
+(** [is_flocal_pred S] asserts that [is_flocal (S x)] holds for any [x].
     It is useful for describing loop invariants. *)
 
-Definition is_local_pred B A (S:A->formula_ B) :=
-  forall x, is_local (S x).
+Definition is_flocal_pred B A (S:A->formula_ B) :=
+  forall x, is_flocal (S x).
 
 
 
 (* ---------------------------------------------------------------------- *)
-(* ** Elimination rules for [is_local] *)
+(* ** Elimination rules for [is_flocal] *)
 
 Section LocalProp.
 Variable (B : Type).
 Implicit Type Q : B->hprop.
 Implicit Type F : formula_ B.
 
-Lemma local_conseq : forall Q' F H Q,
-  is_local F ->
+Lemma flocal_conseq : forall Q' F H Q,
+  is_flocal F ->
   H ==> F Q ->
   Q ===> Q' ->
   H ==> F Q'.
 Proof using.
   introv L M W. rewrite (rm L). hchanges (rm M).
-  unfold local. hsimpl Q. intros r. hchanges W.
+  unfold flocal. hsimpl Q. intros r. hchanges W.
 Qed.
 
-Lemma local_top : forall F H Q,
-  is_local F ->
+Lemma flocal_top : forall F H Q,
+  is_flocal F ->
   H ==> F (Q \*+ \Top) ->
   H ==> F Q.
 Proof using.
-  introv L M. rewrite L. hchanges (rm M). unfold local.
+  introv L M. rewrite L. hchanges (rm M). unfold flocal.
   hsimpl (Q \*+ \Top). hsimpl.
 Qed.
 
-Lemma local_frame : forall H1 H2 F H Q,
-  is_local F ->
+Lemma flocal_frame : forall H1 H2 F H Q,
+  is_flocal F ->
   H ==> H1 \* H2 ->
   H1 ==> F (fun x => H2 \-* Q x) ->
   H ==> F Q.
 Proof using.
   introv L W M. rewrites (rm L). hchanges (rm W). hchanges (rm M).
-  unfold local. hsimpl (fun x => H2 \-* Q x). intros r.
+  unfold flocal. hsimpl (fun x => H2 \-* Q x). intros r.
   hchanges (hwand_cancel H2).
 Qed.
 
-Lemma local_frame_top : forall H1 H2 F H Q,
-  is_local F ->
+Lemma flocal_frame_top : forall H1 H2 F H Q,
+  is_flocal F ->
   H ==> H1 \* H2 ->
   H1 ==> F (fun x => H2 \-* Q x \* \Top) ->
   H ==> F Q.
 Proof using.
-  introv L W M. applys* local_top. applys* local_frame.
+  introv L W M. applys* flocal_top. applys* flocal_frame.
 Qed.
 
 
 (* ---------------------------------------------------------------------- *)
-(* ** Properties of [local] for WP *)
+(* ** Properties of [flocal] for WP *)
 
 (** Local can be erased *)
 
-Lemma local_erase : forall F Q,
-  F Q ==> local F Q.
+Lemma flocal_erase : forall F Q,
+  F Q ==> flocal F Q.
 Proof using.
-  intros. unfold local. repeat hsimpl.
+  intros. unfold flocal. repeat hsimpl.
 Qed.
 
-Lemma local_erase' : forall H F Q,
+Lemma flocal_erase' : forall H F Q,
   H ==> F Q ->
-  H ==> local F Q.
+  H ==> flocal F Q.
 Proof using.
-  introv M. hchanges M. applys local_erase.
+  introv M. hchanges M. applys flocal_erase.
 Qed.
 
-(** Contradictions can be extracted from local formulae *)
+(** Contradictions can be extracted from flocal formulae *)
 
-Lemma local_false : forall F Q,
+Lemma flocal_false : forall F Q,
   (forall Q', F Q' ==> \[False]) ->
-  (local F Q ==> \[False]).
+  (flocal F Q ==> \[False]).
 Proof using.
-  introv M. unfold local. hpull ;=> Q'. hchanges (M Q').
+  introv M. unfold flocal. hpull ;=> Q'. hchanges (M Q').
 Qed.
 
-(** [local] is a covariant transformer w.r.t. predicate inclusion *)
+(** [flocal] is a covariant transformer w.r.t. predicate inclusion *)
 
-Lemma local_weaken : forall F F',
+Lemma flocal_weaken : forall F F',
   F ===> F' ->
-  local F ===> local F'.
+  flocal F ===> flocal F'.
 Proof using.
-  unfold local. introv M. intros Q. hpull ;=> Q'. hsimpl~ Q'.
+  unfold flocal. introv M. intros Q. hpull ;=> Q'. hsimpl~ Q'.
 Qed.
 
-(** [local] can be erased on the left of an entailment if the 
-    formula on the right is local. *)
+(** [flocal] can be erased on the left of an entailment if the 
+    formula on the right is flocal. *)
 
-Lemma local_erase_l : forall F1 F2,
-  is_local F2 ->
+Lemma flocal_erase_l : forall F1 F2,
+  is_flocal F2 ->
   F1 ===> F2 ->
-  local F1 ===> F2.
+  flocal F1 ===> F2.
 Proof using.
-  introv LF M. rewrite LF. intros Q. applys* local_weaken.
+  introv LF M. rewrite LF. intros Q. applys* flocal_weaken.
 Qed.
 
-(** [local] is idempotent, i.e. nested applications
-   of [local] are redundant *)
+(** [flocal] is idempotent, i.e. nested applications
+   of [flocal] are redundant *)
 
-Lemma local_local : forall F,
-  local (local F) = local F.
+Lemma flocal_flocal : forall F,
+  flocal (flocal F) = flocal F.
 Proof using.
   intros F. applys fun_ext_1. intros Q. applys himpl_antisym.
-  { unfold local. hpull ;=> Q' Q''. hsimpl Q''. intros x.
+  { unfold flocal. hpull ;=> Q' Q''. hsimpl Q''. intros x.
     hchanges (qwand_himpl_hwand x Q' (Q \*+ \Top)).
     hchanges (qwand_himpl_hwand x Q'' (Q' \*+ \Top)).
     hchanges (hwand_cancel (Q'' x) (Q' x \* \Top)).
     hchanges (hwand_cancel (Q' x) (Q x \* \Top)). }
     (* LATER: tactic to automate hchanges of hwand_cancel *)
-  { hchanges local_erase. }
+  { hchanges flocal_erase. }
 Qed.
 
-(** A definition whose head is [local] satisfies [is_local] *)
+(** A definition whose head is [flocal] satisfies [is_flocal] *)
 
-Lemma is_local_local : forall F,
-  is_local (local F).
-Proof using. intros. unfolds. rewrite~ local_local. Qed.
+Lemma is_flocal_flocal : forall F,
+  is_flocal (flocal F).
+Proof using. intros. unfolds. rewrite~ flocal_flocal. Qed.
 
-(** Introduction rule for [is_local] on [weakestpre] *)
+(** Introduction rule for [is_flocal] on [weakestpre] *)
 
-Lemma is_local_weakestpre : forall (T:hprop->(B->hprop)->Prop),
+Lemma is_flocal_weakestpre : forall (T:hprop->(B->hprop)->Prop),
   SepBasicSetup.is_local T ->
-  is_local (weakestpre T).
+  is_flocal (weakestpre T).
 Proof using.
-  introv L. unfold is_local. applys fun_ext_1 ;=> Q.
+  introv L. unfold is_flocal. applys fun_ext_1 ;=> Q.
   applys himpl_antisym.
-  { apply~ local_erase'. }
-  { unfold local, wp_triple, weakestpre.
+  { apply~ flocal_erase'. }
+  { unfold flocal, wp_triple, weakestpre.
     hpull ;=> Q' H M. hsimpl (H \* (Q' \--* Q \*+ \Top)).
     xapply M. hsimpl. intros x. hchange (qwand_himpl_hwand x Q' (Q \*+ \Top)).
     hchange (hwand_cancel (Q' x)). hsimpl. }
@@ -246,10 +246,10 @@ End LocalProp.
 (** These auxiliary definitions give the characteristic formula
     associated with each term construct. *)
 
-Definition wp_fail : formula := local (fun Q =>
+Definition wp_fail : formula := flocal (fun Q =>
   \[False]).
 
-Definition wp_val (v:val) : formula := local (fun Q =>
+Definition wp_val (v:val) : formula := flocal (fun Q =>
   Q v).
 
 Definition wp_var (E:ctx) (x:var) : formula :=
@@ -258,10 +258,10 @@ Definition wp_var (E:ctx) (x:var) : formula :=
   | Some v => wp_val v
   end.
 
-Definition wp_let (F1:formula) (F2of:val->formula) : formula := local (fun Q =>
+Definition wp_let (F1:formula) (F2of:val->formula) : formula := flocal (fun Q =>
   F1 (fun X => F2of X Q)).
 
-Definition wp_seq (F1 F2:formula) : formula := local (fun Q =>
+Definition wp_seq (F1 F2:formula) : formula := flocal (fun Q =>
   F1 (fun X => F2 Q)).
 
 Definition wp_getval wp (E:ctx) (t1:trm) (F2of:val->formula) : formula :=
@@ -281,13 +281,13 @@ Definition wp_constr wp (E:ctx) (id:idconstr) : list val -> list trm -> formula 
     | t1::ts' => wp_getval wp E t1 (fun v1 => mk (v1::rvs) ts')
     end.
 
-Definition wp_unop_int (v1:val) (F:int->val) : formula := local (fun Q =>
+Definition wp_unop_int (v1:val) (F:int->val) : formula := flocal (fun Q =>
   \exists n1, \[v1 = val_int n1] \* Q (F n1)).
 
-Definition wp_unop_bool (v1:val) (F:bool->val) : formula := local (fun Q =>
+Definition wp_unop_bool (v1:val) (F:bool->val) : formula := flocal (fun Q =>
   \exists b1, \[v1 = val_bool b1] \* Q (F b1)).
 
-Definition wp_binop_int (v1 v2:val) (F:int->int->val) : formula := local (fun Q =>
+Definition wp_binop_int (v1 v2:val) (F:int->int->val) : formula := flocal (fun Q =>
   \exists n1 n2, \[v1 = val_int n1 /\ v2 = val_int n2] \* Q (F n1 n2)).
 
 Definition wp_apps_val (v0:val) (vs:vals) : formula := 
@@ -299,7 +299,7 @@ Definition wp_apps_val (v0:val) (vs:vals) : formula :=
   | val_prim val_add, (v1::v2::nil) => wp_binop_int v1 v2 (fun n1 n2 => n1 + n2)
   | val_prim val_sub, (v1::v2::nil) => wp_binop_int v1 v2 (fun n1 n2 => n1 - n2)
   | val_prim val_mul, (v1::v2::nil) => wp_binop_int v1 v2 (fun n1 n2 => n1 * n2)
-  | _, _ => local (wp_triple (trm_apps v0 vs))
+  | _, _ => flocal (wp_triple (trm_apps v0 vs))
   end.  (* not included: arithmetic comparisons *)
 
 Definition wp_apps wp (E:ctx) (v0:val) : list val -> list trm -> formula := 
@@ -309,26 +309,26 @@ Definition wp_apps wp (E:ctx) (v0:val) : list val -> list trm -> formula :=
     | t1::ts' => wp_getval wp E t1 (fun v1 => mk (v1::rvs) ts')
     end).
 
-Definition wp_if_val (v:val) (F1 F2:formula) : formula := local (fun Q =>
+Definition wp_if_val (v:val) (F1 F2:formula) : formula := flocal (fun Q =>
   \exists (b:bool), \[v = val_bool b] \* (if b then F1 Q else F2 Q)).
 
 Definition wp_if (F0 F1 F2:formula) : formula :=
   wp_let F0 (fun v => wp_if_val v F1 F2).
 
-Definition wp_while (F1 F2:formula) : formula := local (fun Q =>
+Definition wp_while (F1 F2:formula) : formula := flocal (fun Q =>
   \forall (R:formula),
   let F := wp_if F1 (wp_seq F2 R) (wp_val val_unit) in
-  \[ is_local R /\ F ===> R] \-* (R Q)).
+  \[ is_flocal R /\ F ===> R] \-* (R Q)).
 
-Definition wp_for_val (v1 v2:val) (F1:val->formula) : formula := local (fun Q =>
+Definition wp_for_val (v1 v2:val) (F1:val->formula) : formula := flocal (fun Q =>
   \exists (n1:int) (n2:int), \[v1 = val_int n1 /\ v2 = val_int n2] \*
   \forall (S:int->formula),
   let F i := If (i <= n2) then (wp_seq (F1 i) (S (i+1)))
                           else (wp_val val_unit) in
-  \[ is_local_pred S /\ (forall i, F i ===> S i)] \-* (S n1 Q)).
+  \[ is_flocal_pred S /\ (forall i, F i ===> S i)] \-* (S n1 Q)).
 
 Definition wp_case_val (v:val) (p:pat) (F1of:ctx->formula) (F2:formula) : formula :=
-  local (fun Q => 
+  flocal (fun Q => 
     hand (\forall (G:ctx), \[Ctx.dom G = patvars p /\ v = patsubst G p] \-* F1of G Q)
          (\[forall (G:ctx), Ctx.dom G = patvars p -> v <> patsubst G p] \-* F2 Q) ).
 
@@ -370,17 +370,17 @@ Fixpoint wp (E:ctx) (t:trm) : formula :=
 (* ---------------------------------------------------------------------- *)
 (* ** Properties of semantical wp *)
 
-(** [wp_triple t] is a local formula *)
+(** [wp_triple t] is a flocal formula *)
 
-Lemma is_local_wp_triple : forall t,
-  is_local (wp_triple t).
-Proof using. intros. applys is_local_weakestpre. applys is_local_triple. Qed.
+Lemma is_flocal_wp_triple : forall t,
+  is_flocal (wp_triple t).
+Proof using. intros. applys~ is_flocal_weakestpre. Qed.
 
 (** Equivalence between a [triple] and its weakest-precondition presentation. *)
 
 Lemma triple_eq_himpl_wp_triple : forall H Q t,
   triple t H Q = (H ==> wp_triple t Q).
-Proof using. intros. applys weakestpre_eq. applys is_local_triple. Qed.
+Proof using. intros. applys~ weakestpre_eq. Qed.
 
 (** Reformulation of the right-to-left implication above as an implication. *)
 
@@ -402,31 +402,30 @@ Proof using. introv M. intros Q. rewrite~ <- triple_eq_himpl_wp_triple. Qed.
 
 Lemma triple_wp_triple : forall t Q,
   triple t (wp_triple t Q) Q.
-Proof using. intros. applys weakestpre_pre. applys is_local_triple. Qed.
+Proof using. intros. applys~ weakestpre_pre. Qed.
 
 
 (* ---------------------------------------------------------------------- *)
-(* ** Soundness of the [local] transformer *)
+(* ** Soundness of the [flocal] transformer *)
 
-(** The [local] transformer is sound w.r.t. [triple] *)
+(** The [flocal] transformer is sound w.r.t. [triple] *)
 
-Lemma triple_local_pre : forall t (F:formula) Q,
+Lemma triple_flocal_pre : forall t (F:formula) Q,
   (forall Q, triple t (F Q) Q) ->
-  triple t (local F Q) Q.
+  triple t (flocal F Q) Q.
 Proof using.
-  introv M. rewrite is_local_triple. unfold SepBasicSetup.local.
-  unfold local. hpull ;=> Q'.
-  hsimpl (F Q') ((Q' \--* Q \*+ \Top)) Q'. split.
-  { applys~ M. }
+  introv M. applys~ is_local_elim.
+  unfold flocal. hpull ;=> Q'.
+  hsimpl (F Q') ((Q' \--* Q \*+ \Top)) Q'. split~.
   { hchanges qwand_cancel. }
 Qed.
 
-(** The tactic [remove_local] applies to goal of the form [triple t (local F Q) Q]
+(** The tactic [remove_flocal] applies to goal of the form [triple t (flocal F Q) Q]
     and turns it into [triple t (F Q) Q] for a fresh [Q],  then calls [xpull] *)
 
-Ltac remove_local :=
+Ltac remove_flocal :=
   match goal with |- triple _ _ ?Q =>
-    applys triple_local_pre; try (clear Q; intros Q); xpull; fold wp end.
+    applys triple_flocal_pre; try (clear Q; intros Q); xpull; fold wp end.
 
 
 (* ---------------------------------------------------------------------- *)
@@ -445,7 +444,7 @@ Definition wp_sound t := forall E,
 
 Lemma himpl_wp_fail_l : forall Q H,
   wp_fail Q ==> H.
-Proof using. intros. unfold wp_fail, local. hpull. Qed.
+Proof using. intros. unfold wp_fail, flocal. hpull. Qed.
 
 Lemma qimpl_wp_fail_l : forall F,
   wp_fail ===> F.
@@ -475,10 +474,10 @@ Proof using.
   { destruct C2 as (x&Et). subst. simpl. case_eq (Ctx.lookup x E).
     { intros v Ev. rewrites~ (>> isubst_evalctx_trm_var Ev).
       apply triple_of_wp. applys M2. }
-    { introv N. remove_local. intros; false. } }
+    { introv N. remove_flocal. intros; false. } }
   asserts_rewrite (wp_getval wp E t1 F2of = wp_let (wp E t1) F2of).
   { destruct t1; auto. { false C1. hnfs*. } { false C2. hnfs*. } }
-  remove_local. applys~ triple_isubst_evalctx.
+  remove_flocal. applys~ triple_isubst_evalctx.
   { apply triple_of_wp. applys M1. }
   { intros v. apply triple_of_wp. applys M2. }
 Qed.
@@ -492,7 +491,7 @@ Lemma wp_sound_var : forall x,
 Proof using.
   intros. intros E. applys qimpl_wp_triple. simpl.
   intros Q. unfold wp_var. destruct (Ctx.lookup x E).
-  { remove_local. apply~ triple_val. }
+  { remove_flocal. apply~ triple_val. }
   { applys~ triple_wp_fail. }
 Qed.
 
@@ -500,7 +499,7 @@ Lemma wp_sound_val : forall v,
   wp_sound (trm_val v).
 Proof using.
   intros. intros E. applys qimpl_wp_triple. simpl.
-  intros Q. remove_local. applys~ triple_val.
+  intros Q. remove_flocal. applys~ triple_val.
 Qed.
 
 Lemma wp_sound_fixs : forall f xs t,
@@ -509,7 +508,7 @@ Proof using.
   intros. intros E. applys qimpl_wp_triple. simpl. intros Q.
   destruct xs as [|x xs'].
   { applys~ triple_wp_fail. }
-  { remove_local. applys~ triple_fixs. auto_false. }
+  { remove_flocal. applys~ triple_fixs. auto_false. }
 Qed.
 
 Lemma wp_sound_if_val : forall v0 F1 F2 E t1 t2,
@@ -518,7 +517,7 @@ Lemma wp_sound_if_val : forall v0 F1 F2 E t1 t2,
   wp_if_val v0 F1 F2 ===> wp_triple_ E (trm_if v0 t1 t2).
 Proof using.
   introv M1 M2. applys qimpl_wp_triple. simpl. intros Q.
-  remove_local. intros b ->. applys triple_if_bool.
+  remove_flocal. intros b ->. applys triple_if_bool.
   apply triple_of_wp. case_if*.
 Qed.
 
@@ -529,7 +528,7 @@ Lemma wp_sound_if_trm : forall F1 F2 F3 E t1 t2 t3,
   wp_if F1 F2 F3 ===> wp_triple_ E (trm_if t1 t2 t3).
 Proof using.
   introv M1 M2 M3. applys qimpl_wp_triple. intros Q.
-  simpl. unfold wp_if. remove_local. applys triple_if_trm.
+  simpl. unfold wp_if. remove_flocal. applys triple_if_trm.
   { apply triple_of_wp. applys M1. }
   { intros v. apply triple_of_wp. applys* wp_sound_if_val. }
 Qed.
@@ -551,7 +550,7 @@ Lemma wp_sound_let : forall F1 F2 E x t1 t2,
   wp_let F1 F2 ===> wp_triple_ E (trm_let x t1 t2).
 Proof using.
   introv M1 M2. applys qimpl_wp_triple. simpl. intros Q.
-  remove_local. applys triple_let.
+  remove_flocal. applys triple_let.
   { apply triple_of_wp. applys* M1. }
   { intros X. simpl. apply triple_of_wp.
     rewrite <- isubst_add_eq_subst1_isubst. applys* M2. }
@@ -563,7 +562,7 @@ Lemma wp_sound_seq : forall F1 F2 E t1 t2,
   wp_seq F1 F2 ===> wp_triple_ E (trm_seq t1 t2).
 Proof using.
   introv M1 M2. applys qimpl_wp_triple. simpl. intros Q.
-  remove_local. applys triple_seq.
+  remove_flocal. applys triple_seq.
   { apply triple_of_wp. applys* M1. }
   { intros X. simpl. apply triple_of_wp. applys* M2. }
 Qed.
@@ -573,7 +572,7 @@ Lemma wp_sound_redbinop : forall v op v1 v2,
   wp_val v ===> wp_triple (trm_apps op (trms_vals (v1::v2::nil))).
 Proof using.
   introv M. applys qimpl_wp_triple; intros Q; simpl.
-  remove_local. applys triple_combined.
+  remove_flocal. applys~ is_local_conseq_frame.
   { applys triple_binop M. } { hsimpl. } { hpull ;=> ? ->. hsimpl. }
 Qed.
 
@@ -582,7 +581,7 @@ Lemma wp_sound_redunop_int : forall (F:int->val) op v1,
   wp_unop_int v1 F ===> wp_triple (trm_apps op (trms_vals (v1::nil))).
 Proof using.
   introv M. applys qimpl_wp_triple; intros Q; simpl.
-  remove_local. intros n1 ->. applys triple_combined.
+  remove_flocal. intros n1 ->. applys~ is_local_conseq_frame.
   { applys triple_unop M. } { hsimpl. } { hpull ;=> ? ->. hsimpl. }
 Qed.
 
@@ -591,7 +590,7 @@ Lemma wp_sound_redunop_bool : forall (F:bool->val) op v1,
   wp_unop_bool v1 F ===> wp_triple (trm_apps op (trms_vals (v1::nil))).
 Proof using.
   introv M. applys qimpl_wp_triple; intros Q; simpl.
-  remove_local. intros n1 ->. applys triple_combined.
+  remove_flocal. intros n1 ->. applys~ is_local_conseq_frame.
   { applys triple_unop M. } { hsimpl. } { hpull ;=> ? ->. hsimpl. }
 Qed.
 
@@ -600,7 +599,7 @@ Lemma wp_sound_redbinop_int : forall (F:int->int->val) op v1 v2,
   wp_binop_int v1 v2 F ===> wp_triple (trm_apps op (trms_vals (v1::v2::nil))).
 Proof using.
   introv M. applys qimpl_wp_triple; intros Q; simpl.
-  remove_local. intros n1 n2 (->&->). applys triple_combined.
+  remove_flocal. intros n1 n2 (->&->). applys~ is_local_conseq_frame.
   { applys triple_binop M. } { hsimpl. } { hpull ;=> ? ->. hsimpl. }
 Qed.
 
@@ -609,8 +608,8 @@ Lemma wp_sound_apps_val : forall v0 vs,
 Proof using.
   Hint Constructors redunop redbinop.
   intros.
-  asserts Common: (local (wp_triple (trm_apps v0 vs)) ===> wp_triple (trm_apps v0 vs)).
-  { apply~ local_erase_l. { applys is_local_wp_triple. } }
+  asserts Common: (flocal (wp_triple (trm_apps v0 vs)) ===> wp_triple (trm_apps v0 vs)).
+  { apply~ flocal_erase_l. { applys is_flocal_wp_triple. } }
   intros Q. destruct v0; try solve [ apply Common ].
   rename p into p. destruct p; try solve [ apply Common ];
    destruct vs as [|v1 [|v2 [|]]]; try solve [ apply Common ].
@@ -651,11 +650,11 @@ Lemma wp_sound_while : forall F1 F2 E t1 t2,
   wp_while F1 F2 ===> wp_triple_ E (trm_while t1 t2).
 Proof using.
   introv M1 M2. applys qimpl_wp_triple. simpl. intros Q.
-  remove_local. 
+  remove_flocal. 
   set (R := wp_triple (trm_while (isubst E t1) (isubst E t2))).
   applys triple_hforall R. simpl. applys triple_hwand_hpure_l.
   { split.
-    { applys is_local_wp_triple. }
+    { applys is_flocal_wp_triple. }
     { clears Q. applys qimpl_wp_triple. intros Q.
       applys triple_while_raw. apply~ triple_of_wp.
       applys* wp_sound_if_trm t1 (trm_seq t2 (trm_while t1 t2)) val_unit.
@@ -669,11 +668,11 @@ Lemma wp_sound_for_val : forall (x:var) v1 v2 F1 E t1,
   wp_for_val v1 v2 F1 ===> wp_triple_ E (trm_for x v1 v2 t1).
 Proof using. Opaque Ctx.add Ctx.rem.
   introv M. applys qimpl_wp_triple. simpl. intros Q.
-  remove_local. intros n1 n2 (->&->). 
+  remove_flocal. intros n1 n2 (->&->). 
   set (S := fun (i:int) => wp_triple (isubst E (trm_for x i n2 t1))).
   applys triple_hforall S. simpl. applys triple_hwand_hpure_l.
   { split.
-    { intros r. applys is_local_wp_triple. }
+    { intros r. applys is_flocal_wp_triple. }
     { clears Q. intros i. applys qimpl_wp_triple. intros Q.
       applys triple_for_raw. fold isubst.
       apply~ triple_of_wp. case_if.
@@ -703,7 +702,7 @@ Lemma wp_sound_case_val : forall v1 p F2 F3 t2 t3 E,
   wp_case_val v1 p F2 F3 ===> wp_triple_ E (trm_case v1 p t2 t3).
 Proof using.
   introv M1 M2. applys qimpl_wp_triple. simpl. intros Q.
-  remove_local. applys triple_case.
+  remove_flocal. applys triple_case.
   { intros G HG Hv1. rewrites <- (rm HG).
     applys triple_hand_l. applys triple_hforall G.
     applys~ triple_hwand_hpure_l. apply triple_of_wp.
@@ -734,7 +733,7 @@ Proof using.
   induction ts as [|t ts']; intros.
   { simpl. rewrite List_rev_eq. rew_list. applys qimpl_wp_triple.
     simpl. rewrite List_map_eq.
-    intros Q. remove_local. rewrite map_isubst_trms_vals. applys~ triple_constr. }
+    intros Q. remove_flocal. rewrite map_isubst_trms_vals. applys~ triple_constr. }
   { specializes IHts' __. { intros t' Ht'. applys* IHwp. }
     applys~ wp_sound_getval (fun t1 => trm_constr id (trms_vals (rev rvs) ++ t1 :: ts')).
     intros v1. fold (wp_constr wp E id).
@@ -785,11 +784,11 @@ Qed.
 
 
 (* ---------------------------------------------------------------------- *)
-(* ** All [wp] are trivially local by construction *)
+(* ** All [wp] are trivially flocal by construction *)
 
 Section IsLocalWp.
 
-Hint Extern 1 (is_local _) => (apply is_local_local).
+Hint Extern 1 (is_flocal _) => (apply is_flocal_flocal).
 
 Ltac destruct_lookup :=
   match goal with |- context [Ctx.lookup ?x ?E] => destruct~ (Ctx.lookup x E) end.
@@ -797,32 +796,32 @@ Ltac destruct_lookup :=
 Tactic Notation "destruct_lookup" "~" :=
   destruct_lookup; auto_tilde.
 
-Lemma is_local_wp_getval : forall wp E t1 F2of,
-  is_local (wp E t1) ->
-  (forall v, is_local (F2of v)) ->
-  is_local (wp_getval wp E t1 F2of).
+Lemma is_flocal_wp_getval : forall wp E t1 F2of,
+  is_flocal (wp E t1) ->
+  (forall v, is_flocal (F2of v)) ->
+  is_flocal (wp_getval wp E t1 F2of).
 Proof using.
   introv M1 M2. destruct* t1. { simpl. destruct_lookup~. }
 Qed.
 
-Hint Resolve is_local_wp_getval.
+Hint Resolve is_flocal_wp_getval.
 
-Lemma is_local_wp : forall E t,
-  is_local (wp E t).
+Lemma is_flocal_wp : forall E t,
+  is_flocal (wp E t).
 Proof.
   intros. induction t using trm_induct; try solve [ simpl; eauto ]. 
   { simpl. rename v into x. simpl. unfold wp_var. destruct_lookup~. }
   { simpl. destruct~ xs. }
   { simpl. rename l into ts. simpl. generalize (@nil val) as rvs.
     induction ts as [|t' ts']; intros; auto.
-    { applys* is_local_wp_getval. } }
-  { simpl. applys* is_local_wp_getval. intros v0.
+    { applys* is_flocal_wp_getval. } }
+  { simpl. applys* is_flocal_wp_getval. intros v0.
     rename l into ts. simpl. generalize (@nil val) as rvs.
     induction ts as [|t' ts']; intros; auto.
     { simpl. generalize (List.rev rvs) as vs. intros.
       unfolds wp_apps. destruct~ v0.
       destruct~ p; destruct vs as [|v1 [|v2 [ | ]]]; auto. }
-    { applys* is_local_wp_getval. } }
+    { applys* is_flocal_wp_getval. } }
 Qed.
 
 End IsLocalWp.
